crates/algorithms/sha3/proofs/fstar/extraction/Libcrux_sha3.Traits.fst
@@ -259,32 +259,65 @@ class t_Squeeze2 (v_Self: Type0) (v_T: Type0) = {
 let _ = fun (v_Self:Type0) (v_T:Type0) {|i: t_Squeeze2 v_Self v_T|} -> i._super_i0
 
 /// Trait to squeeze bytes out of the state.
-/// Note that this is implemented for each platform (1, 2, 4) because hax can't
+/// Note that this is implemented for each platform (1, 2, 4) because hax can\'t
 /// handle the mutability required for a generic implementation.
 /// Store blocks `N = 4`
 class t_Squeeze4 (v_Self: Type0) (v_T: Type0) = {
   [@@@ FStar.Tactics.Typeclasses.no_method]_super_i0:t_KeccakItem v_T (mk_usize 4);
   f_squeeze4_pre:
       v_RATE: usize ->
-      v_Self ->
-      t_Slice u8 ->
-      t_Slice u8 ->
-      t_Slice u8 ->
-      t_Slice u8 ->
-      usize ->
-      usize
-    -> Type0;
+      self_: v_Self ->
+      out0: t_Slice u8 ->
+      out1: t_Slice u8 ->
+      out2: t_Slice u8 ->
+      out3: t_Slice u8 ->
+      start: usize ->
+      len: usize
+    -> pred:
+      Type0
+        { Libcrux_sha3.Proof_utils.valid_rate v_RATE && len <=. v_RATE &&
+          ((Rust_primitives.Hax.Int.from_machine start <: Hax_lib.Int.t_Int) +
+            (Rust_primitives.Hax.Int.from_machine len <: Hax_lib.Int.t_Int)
+            <:
+            Hax_lib.Int.t_Int) <=
+          (Rust_primitives.Hax.Int.from_machine (Core_models.Slice.impl__len #u8 out0 <: usize)
+            <:
+            Hax_lib.Int.t_Int) &&
+          (Core_models.Slice.impl__len #u8 out0 <: usize) =.
+          (Core_models.Slice.impl__len #u8 out1 <: usize) &&
+          (Core_models.Slice.impl__len #u8 out0 <: usize) =.
+          (Core_models.Slice.impl__len #u8 out2 <: usize) &&
+          (Core_models.Slice.impl__len #u8 out0 <: usize) =.
+          (Core_models.Slice.impl__len #u8 out3 <: usize) ==>
+          pred };
   f_squeeze4_post:
       v_RATE: usize ->
-      v_Self ->
-      t_Slice u8 ->
-      t_Slice u8 ->
-      t_Slice u8 ->
-      t_Slice u8 ->
-      usize ->
-      usize ->
-      (t_Slice u8 & t_Slice u8 & t_Slice u8 & t_Slice u8)
-    -> Type0;
+      self_: v_Self ->
+      out0: t_Slice u8 ->
+      out1: t_Slice u8 ->
+      out2: t_Slice u8 ->
+      out3: t_Slice u8 ->
+      start: usize ->
+      len: usize ->
+      x: (t_Slice u8 & t_Slice u8 & t_Slice u8 & t_Slice u8)
+    -> pred:
+      Type0
+        { pred ==>
+          (let
+            (out0_future: t_Slice u8),
+            (out1_future: t_Slice u8),
+            (out2_future: t_Slice u8),
+            (out3_future: t_Slice u8) =
+              x
+            in
+            (Core_models.Slice.impl__len #u8 out0_future <: usize) =.
+            (Core_models.Slice.impl__len #u8 out0 <: usize) &&
+            (Core_models.Slice.impl__len #u8 out1_future <: usize) =.
+            (Core_models.Slice.impl__len #u8 out1 <: usize) &&
+            (Core_models.Slice.impl__len #u8 out2_future <: usize) =.
+            (Core_models.Slice.impl__len #u8 out2 <: usize) &&
+            (Core_models.Slice.impl__len #u8 out3_future <: usize) =.
+            (Core_models.Slice.impl__len #u8 out3 <: usize)) };
   f_squeeze4:
       v_RATE: usize ->
       x0: v_Self ->
